VerseRocq/verse/densem/env.v
@@ -1,0 +1,58 @@
+Require Import Imports.
+
+From Stdlib Require Lists.List.
+From Stdlib Require Import Classes.EquivDec.
+Import ssreflect.
+
+Require Import syntax.common.
+Require syntax.mini.
+Require Import PFun.
+Require Import densem.Dom.
+Require Import structures.Sets.
+Import structures.List.
+Import structures.Monad.
+
+Import mini.MiniNotation.
+Import FunctorNotation.
+Import ApplicativeNotation.
+Import MonadNotation.
+Import SetNotations.
+Import List.ListNotations.
+
+Open Scope monad_scope.
+Open Scope list_scope.
+Open Scope mini_expr_scope.
+
+(* --------------- (partial) environments ----------- *)
+
+(* gives a value for *in-scope* identitfiers *)
+(* The denotation of out of scope identifiers is NOT defined. *)
+Definition env := Ident -> option value.
+
+Module Env. 
+
+Definition empty : env := fun x => None.
+
+Definition extend : Ident -> value -> env -> env := 
+  fun x v rho => 
+    fun y => if Nat.eqb x y then Some v else rho y.
+
+End Env.
+
+Declare Scope env_scope.
+Delimit Scope env_scope with env.
+Bind Scope env_scope with env.
+
+Module EnvNotation.
+Notation " x |-> v " := (Env.extend x v Env.empty) (at level 80) : env_scope.
+Notation " x |-> v , e " := (Env.extend x v e) (at level 80, right associativity): env_scope. 
+
+Section NotationExamples.
+Open Scope env_scope.
+Variable x y : Ident.
+Variable v w : value.
+Check  x |-> v.
+Check  x |-> v, y |-> w.
+End NotationExamples.
+
+End EnvNotation.
