VerseRocq/verse/densem/tenv.v
@@ -1,0 +1,71 @@
+Require Import Imports.
+
+From Stdlib Require Lists.List.
+From Stdlib Require Import Classes.EquivDec.
+From Stdlib Require Export FunctionalExtensionality.
+
+Import ssreflect.
+
+Require Import syntax.common.
+Require syntax.mini.
+Require Import PFun.
+Require Import densem.Dom.
+Require Import structures.Sets.
+Import structures.List.
+Import structures.Monad.
+
+Import mini.MiniNotation.
+Import FunctorNotation.
+Import ApplicativeNotation.
+Import MonadNotation.
+Import SetNotations.
+Import List.ListNotations.
+
+Open Scope monad_scope.
+Open Scope list_scope.
+Open Scope mini_expr_scope.
+
+(* --------------- (total) environments ----------- *)
+
+Definition env := Ident -> value.
+
+Module Env.
+
+Definition empty : env := fun x => Dom.Int 0.
+
+Definition extend : Ident -> value -> env -> env := 
+  fun x v rho => 
+    fun y => if Nat.eqb x y then v else rho y.
+
+End Env.
+
+Declare Scope env_scope.
+Delimit Scope env_scope with env.
+Bind Scope env_scope with env.
+
+Module EnvNotation.
+Notation " x |-> v " := (Env.extend x v Env.empty) (at level 80) : env_scope.
+Notation " x |-> v , e " := (Env.extend x v e) (at level 80, right associativity): env_scope. 
+End EnvNotation.
+
+
+Lemma empty_equal r:
+  (forall x, r x = Dom.Int 0) -> 
+  Env.empty = r.
+Proof. 
+  intro h.
+  extensionality x.
+  rewrite h.
+  auto.
+Qed.
+
+Lemma extend_equal r s x v:
+  s x = v -> (forall y, Nat.eqb x y = false -> r y = s y) ->
+  Env.extend x v r = s.
+Proof.
+  intros.
+  extensionality y.
+  unfold Env.extend. destruct (Nat.eqb x y) eqn:E.
+  rewrite PeanoNat.Nat.eqb_eq in E. subst. auto.
+  eauto.
+Qed.
